@prefix owl: <http://www.w3.org/2002/07/owl#> .
@prefix rdfs: <http://www.w3.org/2000/01/rdf-schema#> .
@prefix skos: <http://www.w3.org/2004/02/skos/core#> .
@prefix xsd: <http://www.w3.org/2001/XMLSchema#> .

<http://data.silknow.org/ontology> a owl:Ontology ;
    rdfs:label "SILKNOW Ontology"@en ;
    rdfs:comment "This profile includes the classes and properties used for the SILKNOW project."@en ;
    owl:versionInfo "Exported from OntoME: SILKNOW ongoing"^^xsd:string .

<http://data.silknow.org/T10> a owl:Class ;
    rdfs:label "Ground"@en ;
    rdfs:comment "This class refers to the plain base (or background or field) of the pattern, that is, the underlying part in a composite or decorated textile fabric. It is the cloth used as a basis for embroidery or decoration."^^xsd:string ;
    rdfs:subClassOf <http://www.cidoc-crm.org/cidoc-crm/E22> ;
    skos:notation "T10"^^xsd:string .

<http://data.silknow.org/T11> a owl:Class ;
    rdfs:label "Style"@en ;
    rdfs:comment "This class is used to denote a specific type of style. A style is defined as a set of aesthetic traits that characterize the creations of a school, a nation, an era, or an artist and that allow to date, classify, and evaluate them."^^xsd:string ;
    rdfs:subClassOf <http://www.cidoc-crm.org/cidoc-crm/E55> ;
    skos:notation "T11"^^xsd:string .

<http://data.silknow.org/T12> a owl:Class ;
    rdfs:label "Selvedge (deprecated)"@en ;
    rdfs:comment "This class comprises the longitudinal edge of a textile, often distinguished from the rest of the fabric by its material, weaving or color."^^xsd:string ;
    rdfs:subClassOf <http://www.cidoc-crm.org/cidoc-crm/E22> ;
    skos:notation "T12"^^xsd:string .

<http://data.silknow.org/T13> a owl:Class ;
    rdfs:label "Style Assignment"@en ;
    rdfs:comment "This class comprises the actions of classifying items according to their style."^^xsd:string ;
    rdfs:subClassOf <http://www.cidoc-crm.org/cidoc-crm/E13> ;
    skos:notation "T13"^^xsd:string .

<http://data.silknow.org/T14> a owl:Class ;
    rdfs:label "Starting Border (deprecated)"@en ;
    rdfs:comment "Bla bla bla bla bla bla bla"^^xsd:string ;
    rdfs:subClassOf <http://www.cidoc-crm.org/cidoc-crm/E22> ;
    skos:notation "T14"^^xsd:string .

<http://data.silknow.org/T2> a owl:Class ;
    rdfs:label "Entering (deprecated)"@en ;
    rdfs:comment "This class comprises the act of threading each warp end in the heddles or leashes."^^xsd:string ;
    rdfs:subClassOf <http://www.cidoc-crm.org/cidoc-crm/E29> ;
    skos:notation "T2"^^xsd:string .

<http://data.silknow.org/T22> a owl:Class ;
    rdfs:label "Entering Type (deprecated)"@en ;
    rdfs:comment "This property is used to denote a specific type of entering."^^xsd:string ;
    rdfs:subClassOf <http://www.cidoc-crm.org/cidoc-crm/E55> ;
    skos:notation "T22"^^xsd:string .

<http://data.silknow.org/T24_pattern_unit> a owl:Class ;
    rdfs:label "Pattern Unit"@en ;
    rdfs:comment "The unit which is composed of one or more motifs that, repeated, constitute the pattern of a textile."^^xsd:string ;
    rdfs:subClassOf <http://www.cidoc-crm.org/cidoc-crm/E46> ;
    skos:notation "T24_pattern_unit"^^xsd:string .

<http://data.silknow.org/T27> a owl:Class ;
    rdfs:label "Spinning Type (deprecated)"@en ;
    rdfs:comment """ 
This property is used to denote a specific type of spinning."""^^xsd:string;
    rdfs:subClassOf <http://www.cidoc-crm.org/cidoc-crm/E55> ;
    skos:notation "T27"^^xsd:string .

<http://data.silknow.org/T3> a owl:Class ;
    rdfs:label "Spinning (deprecated)"@en ;
    rdfs:comment "This class comprises the act of producing raw silk yarns from the silkworm cocoons."^^xsd:string ;
    rdfs:subClassOf <http://www.cidoc-crm.org/cidoc-crm/E12> ;
    skos:notation "T3"^^xsd:string .

<http://data.silknow.org/T4> a owl:Class ;
    rdfs:label "Throwing (deprecated)"@en ;
    rdfs:comment """ 
This class comprises the twisting of raw silk yarns. This process produces robuster silk threads, ready to be dyed and woven."""^^xsd:string;
    rdfs:subClassOf <http://www.cidoc-crm.org/cidoc-crm/E12> ;
    skos:notation "T4"^^xsd:string .

<http://data.silknow.org/T8> a owl:Class ;
    rdfs:label "Part Weaving"@en ;
    rdfs:comment "This class comprises one of the actions that results in the production of an instance of T7 Fabric, but this action alone is not sufficient to produce an instance of T7 Fabric. T1 Weaving carried out by instance of E36 Actor can be decomposed into different actions or T8 Part Weaving. Each of them uses different objects and techniques; but they are carried out in parallel and it is their combination that will produce an instance of T7 Fabric."^^xsd:string ;
    rdfs:subClassOf <http://data.silknow.org/T1> ;
    skos:notation "T8"^^xsd:string .

<http://data.silknow.org/T9> a owl:Class ;
    rdfs:label "Pattern Zone"@en ;
    rdfs:comment "This class is used to denote the area of the fabric carrying the pattern."^^xsd:string ;
    rdfs:subClassOf <http://www.cidoc-crm.org/cidoc-crm/E22> ;
    skos:notation "T9"^^xsd:string .

<http://data.silknow.org/L1_assigned_object_type> a owl:ObjectProperty ;
    rdfs:label "Assigned object type"@en ;
    rdfs:comment "This property associates a type with an object."@en ;
    rdfs:domain <http://data.silknow.org/T35_Object_Type_Assignment> ;
    rdfs:range <http://www.cidoc-crm.org/cidoc-crm/E22> ;
    skos:notation "L1_assigned_object_type"^^xsd:string .

<http://data.silknow.org/L10> a owl:ObjectProperty ;
    rdfs:label "used yarn"@en ;
    rdfs:comment "This property is used to associate E12_Production with an instance of E22_Man-Made Object, T15_Yarn."@en ;
    rdfs:domain <http://data.silknow.org/T1> ;
    rdfs:range <http://data.silknow.org/T15> ;
    skos:notation "L10"^^xsd:string .

<http://data.silknow.org/L11> a owl:ObjectProperty ;
    rdfs:label "has weave type"@en ;
    rdfs:comment "This property associates a weave with the type which defines its identity."@en ;
    rdfs:domain <http://data.silknow.org/T21> ;
    rdfs:range <http://data.silknow.org/T32> ;
    skos:notation "L11"^^xsd:string .

<http://data.silknow.org/L12> a owl:ObjectProperty ;
    rdfs:label "has motif type"@en ;
    rdfs:comment "This property associates a motif with the type which defines its identity."@en ;
    rdfs:domain <http://data.silknow.org/T18> ;
    rdfs:range <http://data.silknow.org/T34> ;
    skos:notation "L12"^^xsd:string .

<http://data.silknow.org/L13> a owl:ObjectProperty ;
    rdfs:label "has warping type (deprecated)"@en ;
    rdfs:comment "This property associates a warping with the type which defines its identity."@en ;
    rdfs:domain <http://data.silknow.org/T5> ;
    rdfs:range <http://data.silknow.org/T31> ;
    skos:notation "L13"^^xsd:string .

<http://data.silknow.org/L14> a owl:ObjectProperty ;
    rdfs:label "used specific weaving technique"@en ;
    rdfs:comment "This property associates a textile fibre with the type which defines its identity."@en ;
    rdfs:domain <http://data.silknow.org/T1> ;
    rdfs:range <http://data.silknow.org/T25> ;
    skos:notation "L14"^^xsd:string .

<http://data.silknow.org/L15> a owl:ObjectProperty ;
    rdfs:label "has weft type"@en ;
    rdfs:comment "This property associates a weft with the type which defines its identity."@en ;
    rdfs:domain <http://data.silknow.org/T17> ;
    rdfs:range <http://data.silknow.org/T33> ;
    skos:notation "L15"^^xsd:string .

<http://data.silknow.org/L16> a owl:ObjectProperty ;
    rdfs:label "has woven (deprecated)"@en ;
    rdfs:comment "bbbb"@en ;
    rdfs:domain <http://data.silknow.org/T1> ;
    rdfs:range <http://data.silknow.org/T7> ;
    skos:notation "L16"^^xsd:string .

<http://data.silknow.org/L17> a owl:ObjectProperty ;
    rdfs:label "has loom type"@en ;
    rdfs:comment "This property associates a loom with the type which defines its identity."@en ;
    rdfs:domain <http://data.silknow.org/T6> ;
    rdfs:range <http://data.silknow.org/T26> ;
    skos:notation "L17"^^xsd:string .

<http://data.silknow.org/L2> a owl:ObjectProperty ;
    rdfs:label "has fabric type"@en ;
    rdfs:comment "This property associates a fabric with the type which defines its identity."@en ;
    rdfs:domain <http://data.silknow.org/T7> ;
    rdfs:range <http://data.silknow.org/T23> ;
    skos:notation "L2"^^xsd:string .

<http://data.silknow.org/L3> a owl:ObjectProperty ;
    rdfs:label "has yarn type"@en ;
    rdfs:comment "This property associates a yarn with the type which defines its identity."@en ;
    rdfs:domain <http://data.silknow.org/T15> ;
    rdfs:range <http://data.silknow.org/T28> ;
    skos:notation "L3"^^xsd:string .

<http://data.silknow.org/L4_assigned_domain_type> a owl:ObjectProperty ;
    rdfs:label "Assigned domain type"@en ;
    rdfs:comment "This property associates a domain with an object."@en ;
    rdfs:domain <http://data.silknow.org/T19_Object_Domain_Assignment> ;
    rdfs:range <http://www.cidoc-crm.org/cidoc-crm/E22> ;
    skos:notation "L4_assigned_domain_type"^^xsd:string .

<http://data.silknow.org/L5> a owl:ObjectProperty ;
    rdfs:label "has twist type"@en ;
    rdfs:comment "This property associates a twist with the type which defines its identity."@en ;
    rdfs:domain <http://data.silknow.org/T20> ;
    rdfs:range <http://data.silknow.org/T29> ;
    skos:notation "L5"^^xsd:string .

<http://data.silknow.org/L6> a owl:ObjectProperty ;
    rdfs:label "has warp type"@en ;
    rdfs:comment "This property associates a warp with the type which defines its identity."@en ;
    rdfs:domain <http://data.silknow.org/T16> ;
    rdfs:range <http://data.silknow.org/T30> ;
    skos:notation "L6"^^xsd:string .

<http://data.silknow.org/L7> a owl:ObjectProperty ;
    rdfs:label "used warp"@en ;
    rdfs:comment "This property is used to associate an instance of E12 Production, T1_Weaving, and an instance of E22_Man-Made object, T16_Warp."@en ;
    rdfs:domain <http://data.silknow.org/T1> ;
    rdfs:range <http://data.silknow.org/T16> ;
    skos:notation "L7"^^xsd:string .

<http://data.silknow.org/L8> a owl:ObjectProperty ;
    rdfs:label "used weave"@en ;
    rdfs:comment "This property is used to associate an instance of E12_Production, T1_Weaving, and an instance of E26_Design or Procedure, T21_Weave."@en ;
    rdfs:domain <http://data.silknow.org/T1> ;
    rdfs:range <http://data.silknow.org/T21> ;
    skos:notation "L8"^^xsd:string .

<http://data.silknow.org/L9> a owl:ObjectProperty ;
    rdfs:label "used weft"@en ;
    rdfs:comment "This property is used to associate an instance of E12 Production, T1_Weaving, and an instance of E22_Man-Made object, T17_Weft."@en ;
    rdfs:domain <http://data.silknow.org/T1> ;
    rdfs:range <http://data.silknow.org/T17> ;
    skos:notation "L9"^^xsd:string .

<http://data.silknow.org/T18> a owl:Class ;
    rdfs:label "Motif"@en ;
    rdfs:comment "This class comprises any emblem or pattern that is embroided or stitched on fabrics, cloths, etc. It is any usually recurrent picture used as decoration on textiles."^^xsd:string ;
    rdfs:subClassOf <http://www.cidoc-crm.org/cidoc-crm/E22> ;
    skos:notation "T18"^^xsd:string .

<http://data.silknow.org/T19_Object_Domain_Assignment> a owl:Class ;
    rdfs:label "Object Domain Assignment"@en ;
    rdfs:comment "This class includes actions for the domain classification of heritage objects of all kinds. This action consists in classifying a heritage object in a disciplinary domain expressing the category to which this object belongs. For example: \"textile\" or \"painting. This classification is based on the personal opinion and expertise of the classifier, who will choose to classify this object in a field."^^xsd:string ;
    rdfs:subClassOf <http://www.cidoc-crm.org/cidoc-crm/E17> ;
    skos:notation "T19_Object_Domain_Assignment"^^xsd:string .

<http://data.silknow.org/T20> a owl:Class ;
    rdfs:label "Twist"@en ;
    rdfs:comment "This class comprises the twist of a thread around itself, around its axis, resulting from spinning, twisting, throwing or plying."^^xsd:string ;
    rdfs:subClassOf <http://www.cidoc-crm.org/cidoc-crm/E26> ;
    skos:notation "T20"^^xsd:string .

<http://data.silknow.org/T23> a owl:Class ;
    rdfs:label "Fabric Type"@en ;
    rdfs:comment "This class is used to denote a specific type of textile fabric."^^xsd:string ;
    rdfs:subClassOf <http://www.cidoc-crm.org/cidoc-crm/E55> ;
    skos:notation "T23"^^xsd:string .

<http://data.silknow.org/T25> a owl:Class ;
    rdfs:label "Weaving Technique"@en ;
    rdfs:comment "It refers to the different techniques used in the manufacture of a fabric or textile such as clothing, rugs, tapestries, etc., which are based on the interlacing of textile fibers. Techniques could be divided into those which use a loom or not."^^xsd:string ;
    rdfs:subClassOf <http://www.cidoc-crm.org/cidoc-crm/E29> ;
    skos:notation "T25"^^xsd:string .

<http://data.silknow.org/T26> a owl:Class ;
    rdfs:label "Loom Type"@en ;
    rdfs:comment "This class is used to denote a specific type of loom."^^xsd:string ;
    rdfs:subClassOf <http://www.cidoc-crm.org/cidoc-crm/E55> ;
    skos:notation "T26"^^xsd:string .

<http://data.silknow.org/T28> a owl:Class ;
    rdfs:label "Yarn Type"@en ;
    rdfs:comment "This property is used to denote a specific type of yarn."^^xsd:string ;
    rdfs:subClassOf <http://www.cidoc-crm.org/cidoc-crm/E55> ;
    skos:notation "T28"^^xsd:string .

<http://data.silknow.org/T29> a owl:Class ;
    rdfs:label "Twist Type"@en ;
    rdfs:comment "This class is used to denote a specific type of twist."^^xsd:string ;
    rdfs:subClassOf <http://www.cidoc-crm.org/cidoc-crm/E55> ;
    skos:notation "T29"^^xsd:string .

<http://data.silknow.org/T30> a owl:Class ;
    rdfs:label "Warp Type"@en ;
    rdfs:comment "This class is used to denote a specific type of warp."^^xsd:string ;
    rdfs:subClassOf <http://www.cidoc-crm.org/cidoc-crm/E55> ;
    skos:notation "T30"^^xsd:string .

<http://data.silknow.org/T31> a owl:Class ;
    rdfs:label "Warping Type (deprecated)"@en ;
    rdfs:comment """ 
This property is used to denote a specific type of warping."""^^xsd:string;
    rdfs:subClassOf <http://www.cidoc-crm.org/cidoc-crm/E55> ;
    skos:notation "T31"^^xsd:string .

<http://data.silknow.org/T32> a owl:Class ;
    rdfs:label "Weave Type"@en ;
    rdfs:comment "This class is used to denote a specific type of weave."^^xsd:string ;
    rdfs:subClassOf <http://www.cidoc-crm.org/cidoc-crm/E55> ;
    skos:notation "T32"^^xsd:string .

<http://data.silknow.org/T33> a owl:Class ;
    rdfs:label "Weft Type"@en ;
    rdfs:comment "This class is used to denote a specific type of weft."^^xsd:string ;
    rdfs:subClassOf <http://www.cidoc-crm.org/cidoc-crm/E55> ;
    skos:notation "T33"^^xsd:string .

<http://data.silknow.org/T34> a owl:Class ;
    rdfs:label "Motif Type"@en ;
    rdfs:comment "This class is used to denote a specific type of motif."^^xsd:string ;
    rdfs:subClassOf <http://www.cidoc-crm.org/cidoc-crm/E55> ;
    skos:notation "T34"^^xsd:string .

<http://data.silknow.org/T35_Object_Type_Assignment> a owl:Class ;
    rdfs:label "Object Type Assignment"@en ;
    rdfs:comment "This class includes actions for the classification of heritage objects of all kinds. This classification is based on the expertise and the personal opinion of the classifier."^^xsd:string ;
    rdfs:subClassOf <http://www.cidoc-crm.org/cidoc-crm/E17> ;
    skos:notation "T35_Object_Type_Assignment"^^xsd:string .

<http://data.silknow.org/T5> a owl:Class ;
    rdfs:label "Warping (deprecated)"@en ;
    rdfs:comment "This class comprises the act of creating the warp, by helding the lengthwise warp ends stationary in the same tension on a frame or a loom"^^xsd:string ;
    rdfs:subClassOf <http://www.cidoc-crm.org/cidoc-crm/E12> ;
    skos:notation "T5"^^xsd:string .

<http://data.silknow.org/T6> a owl:Class ;
    rdfs:label "Loom"@en ;
    rdfs:comment "This class comprises a machine or device that facilitates weaving and produces fabric, in which yarn or thread is woven into fabric by the crossing of threads called respectively the warp and weft. Looms, in many formats, hold the warp either vertically or horizontally and can simple or complex elements to adi the weaving process."^^xsd:string ;
    rdfs:subClassOf <http://www.cidoc-crm.org/cidoc-crm/E22> ;
    skos:notation "T6"^^xsd:string .


<http://data.silknow.org/T15> a owl:Class ;
    rdfs:label "Yarn"@en ;
    rdfs:comment "This class comprises thread prepared for weaving or knitting."^^xsd:string ;
    rdfs:subClassOf <http://www.cidoc-crm.org/cidoc-crm/E22> ;
    skos:notation "T15"^^xsd:string .

<http://data.silknow.org/T16> a owl:Class ;
    rdfs:label "Warp"@en ;
    rdfs:comment "This class comprises the longitudinal threads in a textile which are extended lengthwise in the loom, those that are arranged on the loom.."^^xsd:string ;
    rdfs:subClassOf <http://www.cidoc-crm.org/cidoc-crm/E22> ;
    skos:notation "T16"^^xsd:string .

<http://data.silknow.org/T17> a owl:Class ;
    rdfs:label "Weft"@en ;
    rdfs:comment "This class comprises the transverse threads of a textile that crosses from side to side of a web, that is, through the sheds, at right angles to the warp threads with which they are interlaced. The term weft denotes all the picks in a textile."^^xsd:string ;
    rdfs:subClassOf <http://www.cidoc-crm.org/cidoc-crm/E22> ;
    skos:notation "T17"^^xsd:string .

<http://data.silknow.org/T21> a owl:Class ;
    rdfs:label "Weave"@en ;
    rdfs:comment "This class comprises every particular style or manner of interlacing threads passing in one direction with others giving them a concrete angle."^^xsd:string ;
    rdfs:subClassOf <http://www.cidoc-crm.org/cidoc-crm/E55> ;
    skos:notation "T21"^^xsd:string .

<http://data.silknow.org/T7> a owl:Class ;
    rdfs:label "Fabric"@en ;
    rdfs:comment "This class comprises general term to refer to any type of fabric or textile produced by a loom by the regular interweaving of yarns or fibres."^^xsd:string ;
    rdfs:subClassOf <http://www.cidoc-crm.org/cidoc-crm/E22> ;
    skos:notation "T7"^^xsd:string .



<http://data.silknow.org/T1> a owl:Class ;
    rdfs:label "Weaving"@en ;
    rdfs:comment "This class comprises the production process of a fabric. It consist in interlacing the lengthwise threads (warp ends) and the widthwise threads (weft ends) at right angles. The fabric is generally woven on a loom."^^xsd:string ;
    rdfs:subClassOf <http://www.cidoc-crm.org/cidoc-crm/E12> ;
    skos:notation "T1"^^xsd:string .

